formalization/RefinementType.v
@@ -256,26 +256,22 @@ Definition mk_bot ty := {: ty | mk_q_under_bot }.
 Definition mk_top ty := {: ty | mk_q_under_top }.
 Definition mk_eq_var ty (x: atom) := {: ty | b0:x= x }.
 
-(*
-
 Lemma pty_erase_open_eq ρ k s :
-  pty_erase ρ = pty_erase ({k ~p> s} ρ).
+  pty_erase ρ = pty_erase ({k ~p> s} ρ)
+with hty_erase_open_eq τ k s :
+  hty_erase τ = hty_erase ({k ~h> s} τ).
 Proof.
-  induction ρ; eauto.
-  cbn. f_equal. eauto.
+  destruct ρ; simpl; eauto; f_equal; eauto.
+  destruct τ; simpl; eauto.
 Qed.
 
 Lemma pty_erase_subst_eq ρ x s :
-  pty_erase ρ = pty_erase ({x := s}p ρ).
-Proof.
-  induction ρ; eauto.
-  cbn. f_equal. eauto.
-Qed.
-
-Lemma hty_erase_subst_eq τ x s :
+  pty_erase ρ = pty_erase ({x := s}p ρ)
+with hty_erase_subst_eq τ x s :
   hty_erase τ = hty_erase ({x := s}h τ).
 Proof.
-  destruct τ. eauto.
+  destruct ρ; simpl; eauto; f_equal; eauto.
+  destruct τ; simpl; eauto.
 Qed.
 
 Lemma ctx_erase_lookup Γ x ρ :
@@ -323,58 +319,6 @@ Proof.
   by apply not_elem_of_dom.
 Qed.
 
-Lemma subst_fresh_am: forall (a: am) (x:atom) (u: value),
-    x # a -> {x := u}a a = a.
-Proof.
-  intros. induction a; simpl in *; eauto; repeat f_equal;
-    eauto using subst_fresh_qualifier;
-    auto_apply; try my_set_solver.
-Qed.
-
-Lemma subst_fresh_pty: forall (ρ: pty) (x:atom) (u: value),
-    x # ρ -> {x := u}p ρ = ρ.
-Proof.
-  intros.
-  induction ρ using pty_ind';
-    simpl in *; f_equal; eauto using subst_fresh_qualifier.
-  auto_apply. my_set_solver.
-  apply subst_fresh_am. my_set_solver.
-  rewrite <- map_id.
-  apply map_ext_Forall.
-
-  (* A better proof is probably first show [x ∉ ⋃ map ... post] is equivalent to
-  [Forall (fun ... => x ∉ ...) post] (something like
-  [union_list_subseteq_not_in]), and then go from there. But don't bother yet. *)
-  induction post; eauto.
-  simp_hyps. simpl in *.
-  decompose_Forall_hyps.
-  econstructor. simpl.
-  f_equal.
-  apply subst_fresh_am. my_set_solver.
-  auto_apply. my_set_solver.
-  auto_apply. set_solver. eauto.
-Qed.
-
-Lemma subst_fresh_postam: forall (pa: postam) (x:atom) (u: value),
-    x # pa -> {x := u}pa pa = pa.
-Proof.
-  induction pa; eauto; intros.
-  destruct a. simpl in *.
-  repeat f_equal.
-  apply subst_fresh_am. my_set_solver.
-  apply subst_fresh_pty. my_set_solver.
-  auto_apply. my_set_solver.
-Qed.
-
-Lemma subst_fresh_hty: forall (τ: hty) (x:atom) (u: value),
-    x # τ -> {x := u}h τ = τ.
-Proof.
-  destruct τ. simpl. intros.
-  f_equal.
-  apply subst_fresh_am. my_set_solver.
-  apply subst_fresh_postam. my_set_solver.
-Qed.
-
 Lemma subst_commute_am : forall x u_x y u_y a,
     x <> y -> x ∉ fv_value u_y -> y ∉ fv_value u_x ->
     {x := u_x }a ({y := u_y }a a) = {y := u_y }a ({x := u_x }a a).
@@ -385,33 +329,35 @@ Qed.
 
 Lemma subst_commute_pty : forall x u_x y u_y ρ,
     x <> y -> x ∉ fv_value u_y -> y ∉ fv_value u_x ->
-    {x := u_x }p ({y := u_y }p ρ) = {y := u_y }p ({x := u_x }p ρ).
+    {x := u_x }p ({y := u_y }p ρ) = {y := u_y }p ({x := u_x }p ρ)
+with subst_commute_hty : forall x u_x y u_y τ,
+    x <> y -> x ∉ fv_value u_y -> y ∉ fv_value u_x ->
+    {x := u_x }h ({y := u_y }h τ) = {y := u_y }h ({x := u_x }h τ).
 Proof.
-  intros.
-  induction ρ using pty_ind'; simpl; f_equal;
+  destruct ρ; simpl; intros; f_equal;
     eauto using subst_commute_qualifier, subst_commute_am.
-  rewrite !map_map. simpl.
-  apply map_ext_Forall.
-  eapply Forall_impl; eauto. intros [] **. simpl.
-  f_equal; eauto using subst_commute_am.
+  destruct τ; simpl; intros; f_equal;
+    eauto using subst_commute_qualifier, subst_commute_am.
 Qed.
 
-Lemma subst_commute_postam : forall x u_x y u_y pa,
-    x <> y -> x ∉ fv_value u_y -> y ∉ fv_value u_x ->
-    {x := u_x }pa ({y := u_y }pa pa) = {y := u_y }pa ({x := u_x }pa pa).
+Lemma subst_fresh_am: forall (a: am) (x:atom) (u: value),
+    x # a -> {x := u}a a = a.
 Proof.
-  intros.
-  induction pa; simpl; f_equal; eauto.
-  f_equal; eauto using subst_commute_pty, subst_commute_am.
+  intros. induction a; simpl in *; eauto; repeat f_equal;
+    eauto using subst_fresh_qualifier;
+    auto_apply; try my_set_solver.
 Qed.
 
-Lemma subst_commute_hty : forall x u_x y u_y e,
-    x <> y -> x ∉ fv_value u_y -> y ∉ fv_value u_x ->
-    {x := u_x }h ({y := u_y }h e) = {y := u_y }h ({x := u_x }h e).
+Lemma subst_fresh_pty: forall (ρ: pty) (x:atom) (u: value),
+    x # ρ -> {x := u}p ρ = ρ
+with subst_fresh_hty: forall (τ: hty) (x:atom) (u: value),
+    x # τ -> {x := u}h τ = τ.
 Proof.
-  intros.
-  destruct e. simpl.
-  rewrite subst_commute_am, subst_commute_postam; eauto.
+  destruct ρ; simpl; intros; f_equal; eauto using subst_fresh_qualifier;
+    auto_apply; my_set_solver.
+  destruct τ; simpl; intros; f_equal;
+    solve [ auto_apply; my_set_solver
+          | apply subst_fresh_am; my_set_solver ].
 Qed.
 
 Lemma open_fv_am' (a : am) (v : value) k :
@@ -422,24 +368,15 @@ Proof.
 Qed.
 
 Lemma open_fv_pty' (ρ : pty) (v : value) k :
-  pty_fv ρ ⊆ pty_fv ({k ~p> v} ρ).
+  pty_fv ρ ⊆ pty_fv ({k ~p> v} ρ)
+with open_fv_hty' (τ : hty) (v : value) k :
+  hty_fv τ ⊆ hty_fv ({k ~h> v} τ).
 Proof.
-  revert k.
-  induction ρ using pty_ind'; intros; simpl; eauto using open_fv_qualifier'.
-  repeat apply union_mono; eauto using open_fv_am'.
-  rewrite map_map. simpl.
-  apply union_list_mono.
-  clear - H.
-  (* Should have a [Forall] to [Forall2] lemma, or something about [Forall2] and
-  [map]. *)
-  induction post; simpl.
-  econstructor.
-  destruct a. simpl.
-  econstructor.
-  apply union_mono. eauto using open_fv_am'.
-  sinvert H. eauto.
-  apply IHpost.
-  sinvert H. eauto.
+  all: revert k.
+  destruct ρ; simpl; intros; eauto using open_fv_qualifier';
+    repeat apply union_mono; eauto.
+  destruct τ; simpl; intros;
+    repeat apply union_mono; eauto using open_fv_am'.
 Qed.
 
 Lemma remove_arr_pty_ctx_dom_union Γ Γ' :
@@ -461,17 +398,14 @@ Qed.
 Lemma remove_arr_pty_ctx_dom_singleton x v :
   ctxdom ⦑ [(x, v)] ⦒ ⊆ {[x]}.
 Proof.
-  simpl. case_split. simpl. my_set_solver.
-  simpl. my_set_solver.
+  simpl. case_split; simpl; my_set_solver.
 Qed.
 
 Lemma remove_arr_pty_ctx_dom_subseteq Γ :
   ctxdom ⦑ Γ ⦒ ⊆ ctxdom Γ.
 Proof.
   induction Γ; intros; simpl. my_set_solver.
-  repeat case_split; simpl.
-  my_set_solver.
-  my_set_solver.
+  repeat case_split; simpl; my_set_solver.
 Qed.
 
 Lemma open_subst_same_qualifier: forall x y (ϕ : qualifier) k,
@@ -508,74 +442,18 @@ Proof.
   qsimpl.
 Qed.
 
-Lemma postam_open_in (pa : postam) B ρ v_x k :
-  In (B, ρ) ({k ~pa> v_x} pa) ->
-  exists B' ρ', In (B', ρ') pa /\ B = {k ~a> v_x} B' /\ ρ = {k ~p> v_x} ρ'.
-Proof.
-  induction pa; simpl; intros; qauto.
-Qed.
-
-Lemma postam_in_open (pa : postam) B ρ v_x k :
-  In (B, ρ) pa ->
-  In ({k ~a> v_x} B, {k ~p> v_x} ρ) ({k ~pa> v_x} pa).
-Proof.
-  induction pa; simpl; intros; qauto.
-Qed.
-
-Lemma postam_subst_in (pa : postam) B ρ v_x x :
-  In (B, ρ) ({x := v_x}pa pa) ->
-  exists B' ρ', In (B', ρ') pa /\ B = {x := v_x}a B' /\ ρ = {x := v_x}p ρ'.
-Proof.
-  induction pa; simpl; intros; qauto.
-Qed.
-
-Lemma postam_in_subst (pa : postam) B ρ v_x x :
-  In (B, ρ) pa ->
-  In ({x := v_x}a B, {x := v_x}p ρ) ({x := v_x}pa pa).
-Proof.
-  induction pa; simpl; intros; qauto.
-Qed.
-
 Lemma open_subst_same_pty: forall x y (ρ : pty) k,
     x # ρ ->
-    {x := y }p ({k ~p> x} ρ) = {k ~p> y} ρ.
-Proof.
-  induction ρ using pty_ind'; cbn; intros; eauto.
-  f_equal. eauto using open_subst_same_qualifier.
-  f_equal. auto_apply. my_set_solver.
-  apply open_subst_same_am. my_set_solver.
-  rewrite map_map. apply map_ext_in.
-  intros [] **.
-  simpl_union H0.
-  eapply not_in_union_list in Hfresh0; eauto using in_map.
-  cbn in *. f_equal. apply open_subst_same_am. my_set_solver.
-  eapply Forall_forall in H; eauto. apply H.
-  my_set_solver.
-Qed.
-
-Lemma open_subst_same_postam: forall x y (pa : postam) k,
-    x # pa ->
-    {x := y }pa ({k ~pa> x} pa) = {k ~pa> y} pa.
-Proof.
-  induction pa; intros; eauto.
-  destruct a. cbn in *.
-  f_equal. f_equal. apply open_subst_same_am. my_set_solver.
-  apply open_subst_same_pty. my_set_solver.
-  rewrite map_map. apply map_ext_in.
-  intros [] **. cbn.
-  simpl_union H.
-  eapply not_in_union_list in Hfresh0; eauto using in_map.
-  f_equal. apply open_subst_same_am. my_set_solver.
-  apply open_subst_same_pty. my_set_solver.
-Qed.
-
-Lemma open_subst_same_hty: forall x y (τ : hty) k,
+    {x := y }p ({k ~p> x} ρ) = {k ~p> y} ρ
+with open_subst_same_hty: forall x y (τ : hty) k,
     x # τ ->
     {x := y }h ({k ~h> x} τ) = {k ~h> y} τ.
 Proof.
-  destruct τ. cbn. intros.
-  f_equal. apply open_subst_same_am. my_set_solver.
-  apply open_subst_same_postam. my_set_solver.
+  destruct ρ; simpl; intros; f_equal; eauto using open_subst_same_qualifier;
+    auto_apply; my_set_solver.
+  destruct τ; simpl; intros; f_equal;
+    solve [ auto_apply; my_set_solver
+          | apply open_subst_same_am; my_set_solver ].
 Qed.
 
 Lemma subst_open_qualifier: forall (ϕ: qualifier) (x:atom) (u: value) (w: value) (k: nat),
@@ -601,32 +479,12 @@ Proof.
 Qed.
 
 Lemma subst_open_pty: forall (ρ: pty) (x:atom) (u: value) (w: value) (k: nat),
-    lc w -> {x := w}p ({k ~p> u} ρ) = ({k ~p> {x := w}v u} ({x := w}p ρ)).
-Proof.
-  induction ρ using pty_ind'; cbn; intros.
-  f_equal. eauto using subst_open_qualifier.
-  f_equal; eauto using subst_open_am.
-  rewrite !map_map. apply map_ext_in.
-  intros [] **. cbn. f_equal. eauto using subst_open_am.
-  eapply Forall_forall in H; eauto.
-  eauto.
-Qed.
-
-Lemma subst_open_postam: forall (pa: postam) (x:atom) (u: value) (w: value) (k: nat),
-    lc w -> {x := w}pa ({k ~pa> u} pa) = ({k ~pa> {x := w}v u} ({x := w}pa pa)).
-Proof.
-  induction pa; cbn; intros; eauto.
-  destruct a. cbn. f_equal. f_equal.
-  eauto using subst_open_am. eauto using subst_open_pty.
-  rewrite !map_map. apply map_ext_in.
-  intros [] **. cbn. f_equal; eauto using subst_open_am, subst_open_pty.
-Qed.
-
-Lemma subst_open_hty: forall (τ: hty) (x:atom) (u: value) (w: value) (k: nat),
+    lc w -> {x := w}p ({k ~p> u} ρ) = ({k ~p> {x := w}v u} ({x := w}p ρ))
+with subst_open_hty: forall (τ: hty) (x:atom) (u: value) (w: value) (k: nat),
     lc w -> {x := w}h ({k ~h> u} τ) = ({k ~h> {x := w}v u} ({x := w}h τ)).
 Proof.
-  intros. destruct τ.
-  simpl. f_equal; eauto using subst_open_am, subst_open_postam.
+  destruct ρ; simpl; intros; f_equal; eauto using subst_open_qualifier.
+  destruct τ; simpl; intros; f_equal; eauto using subst_open_am.
 Qed.
 
 Lemma subst_open_qualifier_closed:
@@ -644,15 +502,6 @@ Lemma subst_open_pty_closed:
     lc w → {x := w }p ({k ~p> u} ρ) = {k ~p> u} ({x := w }p ρ).
 Proof.
   intros. rewrite subst_open_pty; auto.
-  rewrite (subst_fresh_value); eauto. set_solver.
-Qed.
-
-Lemma subst_open_postam_closed:
-  ∀ (pa : postam) (x : atom) (u w : value) (k : nat),
-    closed_value u ->
-    lc w → {x := w }pa ({k ~pa> u} pa) = {k ~pa> u} ({x := w }pa pa).
-Proof.
-  intros. rewrite subst_open_postam; auto.
   rewrite (subst_fresh_value); eauto. set_solver.
 Qed.
 
@@ -707,6 +556,13 @@ Proof.
   rewrite subst_open_pty; auto. simpl. rewrite decide_False; auto.
 Qed.
 
+Lemma subst_open_var_hty: forall x y (u: value) (τ: hty) (k: nat),
+    x <> y -> lc u -> {x := u}h ({k ~h> y} τ) = ({k ~h> y} ({x := u}h τ)).
+Proof.
+  intros.
+  rewrite subst_open_hty; auto. simpl. rewrite decide_False; auto.
+Qed.
+
 Lemma subst_lc_am : forall x (u: value) (a: am),
     lc_am a -> lc u -> lc_am ({x := u}a a).
 Proof.
@@ -720,33 +576,16 @@ Proof.
 Qed.
 
 Lemma subst_lc_pty : forall x (u: value) (ρ: pty),
-    lc_pty ρ -> lc u -> lc_pty ({x := u}p ρ).
-Proof.
-  induction 1; intros.
-  econstructor. instantiate_atom_listctx.
-  - apply_eq subst_lc_qualifier; eauto.
-    apply subst_open_var_qualifier; eauto; my_set_solver.
-  - simpl. econstructor; eauto.
-    instantiate_atom_listctx.
-    rewrite <- subst_open_var_am by (eauto; my_set_solver).
-    eauto using subst_lc_am.
-    intros x0 **. repeat specialize_with x0.
-    rewrite in_map_iff in H6. simp_hyps. simpl in *.
-    rewrite <- subst_open_var_am by (eauto; my_set_solver).
-    eauto using subst_lc_am.
-    intros x0 **. repeat specialize_with x0.
-    rewrite in_map_iff in H6. simp_hyps. simpl in *.
-    rewrite <- subst_open_var_pty by (eauto; my_set_solver).
-    eauto.
-Qed.
-
-Lemma subst_lc_hty : forall x (u: value) (τ: hty),
+    lc_pty ρ -> lc u -> lc_pty ({x := u}p ρ)
+with subst_lc_hty : forall x (u: value) (τ: hty),
     lc_hty τ -> lc u -> lc_hty ({x := u}h τ).
 Proof.
-  induction 1. intros.
-  econstructor. eauto using subst_lc_am.
-  intros. apply postam_subst_in in H3. simp_hyps. subst. eauto using subst_lc_am.
-  intros. apply postam_subst_in in H3. simp_hyps. subst. eauto using subst_lc_pty.
+  all: destruct 1; intros; simpl; econstructor; eauto using subst_lc_am;
+    instantiate_atom_listctx.
+  - rewrite <- subst_open_var_qualifier by (eauto; my_set_solver);
+      eauto using subst_lc_qualifier.
+  - rewrite <- subst_open_var_hty by (eauto; my_set_solver); eauto.
+  - rewrite <- subst_open_var_pty by (eauto; my_set_solver); eauto.
 Qed.
 
 Lemma fv_of_subst_qualifier:
@@ -770,25 +609,16 @@ Qed.
 
 Lemma fv_of_subst_pty:
   forall x (u : value) (ρ: pty),
-    pty_fv ({x := u }p ρ) ⊆ (pty_fv ρ ∖ {[x]}) ∪ fv_value u.
+    pty_fv ({x := u }p ρ) ⊆ (pty_fv ρ ∖ {[x]}) ∪ fv_value u
+with fv_of_subst_hty:
+  forall x (u : value) (τ: hty),
+    hty_fv ({x := u }h τ) ⊆ (hty_fv τ ∖ {[x]}) ∪ fv_value u.
 Proof.
-  induction ρ using pty_ind'; simpl.
-  eauto using fv_of_subst_qualifier.
-  rewrite map_map. simpl.
-  etrans.
-  repeat apply union_mono.
-  eauto.
-  apply fv_of_subst_am.
-  instantiate (1:=⋃ map (λ e : am * pty, am_fv e.1 ∪ pty_fv e.2) post ∖ {[x]} ∪ fv_value u).
-  2 : my_set_solver.
-  clear - H.
-  induction post; simpl. my_set_solver.
-  destruct a. sinvert H. simp_hyps. simpl in *.
-  etrans.
-  repeat apply union_mono.
-  apply fv_of_subst_am.
-  eauto. eauto.
-  my_set_solver.
+  destruct ρ; simpl; intros; eauto using fv_of_subst_qualifier.
+  etrans. apply union_mono; eauto. my_set_solver.
+  destruct τ; simpl; intros.
+  etrans. repeat apply union_mono; eauto using fv_of_subst_am. my_set_solver.
+  etrans. repeat apply union_mono; eauto using fv_of_subst_am. my_set_solver.
 Qed.
 
 Lemma fv_of_subst_pty_closed:
@@ -798,33 +628,6 @@ Lemma fv_of_subst_pty_closed:
 Proof.
   intros.
   rewrite fv_of_subst_pty.
-  my_set_solver.
-Qed.
-
-Lemma fv_of_subst_postam:
-  forall x (u : value) (pa: postam),
-    postam_fv ({x := u }pa pa) ⊆ (postam_fv pa ∖ {[x]}) ∪ fv_value u.
-Proof.
-  induction pa; simpl; eauto. my_set_solver.
-  destruct a. simpl in *.
-  cbn.
-  etrans.
-  repeat apply union_mono.
-  apply fv_of_subst_am.
-  apply fv_of_subst_pty.
-  eauto.
-  my_set_solver.
-Qed.
-
-Lemma fv_of_subst_hty:
-  forall x (u : value) (τ: hty),
-    hty_fv ({x := u }h τ) ⊆ (hty_fv τ ∖ {[x]}) ∪ fv_value u.
-Proof.
-  destruct τ. simpl.
-  etrans.
-  apply union_mono.
-  apply fv_of_subst_am.
-  apply fv_of_subst_postam.
   my_set_solver.
 Qed.
 
@@ -861,42 +664,17 @@ Qed.
 
 Lemma open_not_in_eq_pty (x : atom) (ρ : pty) k :
   x # {k ~p> x} ρ ->
-  forall e, ρ = {k ~p> e} ρ.
-Proof.
-  revert k.
-  induction ρ using pty_ind'; simpl; intros.
-  f_equal. eapply open_not_in_eq_qualifier. my_set_solver.
-  f_equal. auto_apply. my_set_solver.
-  apply open_not_in_eq_am with (x:=x). my_set_solver.
-  (* Again, an induction here is quite ugly. *)
-  induction post; simpl; intros; eauto.
-  sinvert H.
-  destruct a. simpl in *.
-  repeat f_equal.
-  apply open_not_in_eq_am with x. my_set_solver.
-  auto_apply. my_set_solver.
-  auto_apply; eauto. my_set_solver.
-Qed.
-
-Lemma open_not_in_eq_postam (x : atom) (pa : postam) k :
-  x # {k ~pa> x} pa ->
-  forall e, pa = {k ~pa> e} pa.
-Proof.
-  induction pa; simpl; intros; eauto.
-  destruct a. simpl in *.
-  repeat f_equal.
-  apply open_not_in_eq_am with x. my_set_solver.
-  apply open_not_in_eq_pty with x. my_set_solver.
-  auto_apply. my_set_solver.
-Qed.
-
-Lemma open_not_in_eq_hty (x : atom) (τ : hty) k :
+  forall e, ρ = {k ~p> e} ρ
+with open_not_in_eq_hty (x : atom) (τ : hty) k :
   x # {k ~h> x} τ ->
-  τ = {k ~h> x} τ.
+  forall e, τ = {k ~h> e} τ.
 Proof.
-  destruct τ. simpl. intros.
-  f_equal. apply open_not_in_eq_am with x. my_set_solver.
-  apply open_not_in_eq_postam with x. my_set_solver.
+  all: revert k; specialize (open_not_in_eq_pty x); specialize (open_not_in_eq_hty x).
+  destruct ρ; simpl; intros; f_equal; eauto using open_not_in_eq_qualifier;
+    auto_apply; my_set_solver.
+  destruct τ; simpl; intros; f_equal;
+    solve [ auto_apply; my_set_solver
+          | apply (open_not_in_eq_am x); my_set_solver ].
 Qed.
 
 Lemma subst_intro_pty: forall (ρ: pty) (x:atom) (w: value) (k: nat),
@@ -939,30 +717,25 @@ Proof.
   eauto using lc_subst_qualifier.
 Qed.
 
-Lemma lc_subst_pty: forall x (u: value) (ρ: pty), lc_pty ({x := u}p ρ) -> lc u -> lc_pty ρ.
+Lemma lc_subst_pty: forall x (u: value) (ρ: pty), lc_pty ({x := u}p ρ) -> lc u -> lc_pty ρ
+with lc_subst_hty: forall x (u: value) (τ: hty), lc_hty ({x := u}h τ) -> lc u -> lc_hty τ.
 Proof.
   intros.
   remember (({x:=u}p) ρ).
   generalize dependent ρ.
-  induction H; intros.
-  - destruct ρ; simpl in *; simplify_eq.
-    econstructor.
+  destruct H; intros ρ' **; destruct ρ'; simpl in *; simplify_eq;
+    econstructor; eauto;
     instantiate_atom_listctx.
-    rewrite <- subst_open_var_qualifier in * by (eauto; my_set_solver).
+  rewrite <- subst_open_var_qualifier in * by (eauto; my_set_solver);
     eauto using lc_subst_qualifier.
-  - destruct ρ0; simpl in *; simplify_eq.
-    econstructor; eauto.
-    instantiate_atom_listctx.
-    rewrite <- subst_open_var_am in * by (eauto; my_set_solver).
-    eauto using lc_subst_am.
-    intros. repeat specialize_with x0.
-    eapply postam_in_subst in H6. eapply H2 in H6.
-    rewrite <- subst_open_var_am in * by (eauto; my_set_solver).
-    eauto using lc_subst_am.
-    intros. repeat specialize_with x0.
-    eapply H4. eauto using postam_in_subst.
-    rewrite <- subst_open_var_pty in * by (eauto; my_set_solver).
-    eauto.
+  rewrite <- subst_open_var_hty in * by (eauto; my_set_solver); eauto.
+  rewrite <- subst_open_var_pty in * by (eauto; my_set_solver); eauto.
+
+  intros.
+  remember (({x:=u}h) τ).
+  generalize dependent τ.
+  destruct H; intros τ' **; destruct τ'; simpl in *; simplify_eq;
+    econstructor; eauto using lc_subst_am.
 Qed.
 
 Lemma open_rec_lc_qualifier: forall (v: value) (ϕ: qualifier) (k: nat),
@@ -1028,4 +801,11 @@ Proof.
   simpl. eauto using open_lc_respect_value.
 Qed.
 
-*)
+Lemma closed_pty_subseteq_proper s1 s2 ρ :
+  closed_pty s1 ρ ->
+  s1 ⊆ s2 ->
+  closed_pty s2 ρ.
+Proof.
+  intros. sinvert H. split. eauto.
+  my_set_solver.
+Qed.
